Document and rename environment lookup tactics.

rocq-osiris/theories/proofmode/env_lookups.v
@@ -6,63 +6,128 @@ From osiris.program_logic Require Import program_logic.
 From osiris.tactics Require Import utils iris_bindings.
 From osiris.proofmode Require Import equality.
 
+(* This file defines the [imp_path] tactic, used for solving goals of the
+   form [imp (eval η (EPath p)) {{ Φ }}]. *)
+
 (* --------------------------------------------------------------------------*)
-(* The following part defines module specifications. *)
+(* Specifications for whole modules. *)
 
-Lemma lookup_name_nil name :
-  lookup_name [] name = None.
-Proof. reflexivity. Qed.
-
-Lemma lookup_name_app_l name xs ys a :
-  lookup_name xs name = Some a →
-  lookup_name (xs ++ ys) name = Some a.
-Proof.
-  induction xs as [|[x v] xs IH].
-  - rewrite lookup_name_nil. discriminate 1.
-  - simpl.
-    destruct (name =? x)%string.
-    + inversion 1; by subst.
-    + apply IH.
-Qed.
-
-Lemma lookup_name_app_r name xs ys :
-  lookup_name xs name = None →
-  lookup_name (xs ++ ys) name = lookup_name ys name.
-Proof.
-  induction xs as [|[x v] xs IH].
-  - auto.
-  - simpl.
-    destruct (name =? x)%string.
-    + discriminate 1.
-    + apply IH.
-Qed.
-
-Section Modules.
+Section ModuleSpecs.
   Context `{!osirisGS Σ}.
 
-  (* Specification over a whole path. *)
+  (* Specification over a path:
+     [path_spec p Φ η] states that in environment [η],
+     [p] resolves to some value [#x], and that [Φ x] holds. *)
+  Definition path_spec `{Encode A} (p : path) (Φ : A → iProp Σ) (η : env) : iProp Σ :=
+    ∃ x, ⌜lookup_path η p = Some #x⌝ ∗ Φ x.
 
-  Definition path_spec `{Encode A} (p : path) (spec : A → iProp Σ) (η : env) : iProp Σ :=
-    ∃ x, ⌜lookup_path η p = Some #x⌝ ∗ spec x.
+  (* Specification over a name - aka a singleton path. *)
+  Definition in_env `{Encode A} (name : var) (Φ : A → iProp Σ) (η : env) : iProp Σ :=
+    ∃ x, ⌜lookup_name η name = Some #x⌝ ∗ Φ x.
 
-  (* Specification over a variable name. *)
+  (* A pure variant of [in_env], in Prop. *)
+  Definition pure_in_env `{Encode A} (name : var) (Φ : A → Prop) (η : env) : Prop :=
+    ∃ x, lookup_name η name = Some #x ∧ Φ x.
 
-  Definition in_env `{Encode A} (name : var) (spec : A → iProp Σ) (η : env) : iProp Σ :=
-    ∃ x, ⌜lookup_name η name = Some #x⌝ ∗ spec x.
+  (* We use [enc_spec] to represent postconditions ([enc_spec.spec])
+     over arbitary encodable types ([enc_spec.res_type]). *)
+  Record enc_spec {PROP : Type} :=
+    is_spec
+      {
+        res_type : Type;
+        res_type_enc : Encode res_type;
+        spec : res_type → PROP;
+      }.
+  (* Make it so [enc_spec] displays as [has_spec name Φ]. *)
+  Global Arguments enc_spec {_}.
+  Global Arguments res_type {_}.
+  Global Arguments res_type_enc {_}.
+  Global Arguments spec {_}.
+  Global Arguments is_spec {_ _ _}.
+  Global Add Printing Constructor enc_spec.
 
-  Definition pure_in_env `{Encode A} (name : var) (spec : A → Prop) (η : env) : Prop :=
-    ∃ x, lookup_name η name = Some #x ∧ spec x.
+  Instance dom_env : Dom (env) (gset var) := λ η, list_to_set (η.*1).
 
-  Lemma var_spec_app `{Encode A} x (Φ : A → iProp Σ) δ η :
-    in_env x Φ δ -∗
-    in_env x Φ (δ ++ η).
+  (* [context (zip xs Φs) d η] is a specification over an environment [η].
+
+     It states that every name in [xs] is bound to some value in [η],
+     and this variable persistently satisfies the corresponding
+     postcondition in [Φs].
+
+     Additionally, [context] states [η]'s domain is [d]. *)
+
+  Definition context (specs : list (var * @enc_spec (iProp Σ))) d : env → iProp Σ :=
+    λ η, (⌜dom η = d⌝ ∗
+           [∗ list] '(x, s) ∈ specs,
+            @in_env s.(res_type) s.(res_type_enc) x (λ res, □ s.(spec) res) η)%I.
+
+  (* Because all of the specifications in [context] hold persistently,
+     [context] is persistent. *)
+  Global Instance context_pers specs d η : Persistent (context specs d η).
+  Proof. apply _. Qed.
+
+  (* A rephrasing of [context] in a pure context. *)
+  Definition pure_context (specs : list (name * @enc_spec Prop)) d : env → Prop :=
+    λ η, dom η = d ∧
+         Forall (λ '(x, s),
+                   @pure_in_env s.(res_type) s.(res_type_enc) x s.(spec) η) specs.
+
+  (* [var_spec] acts as a smart constructor for a pair of a variable
+     and its specification. *)
+  Definition var_spec {PROP} `{Encode A} (x : var) (Φ : A → PROP) : var * (@enc_spec PROP) :=
+    (x, is_spec Φ).
+
+  (* Check *)
+  (*   context [ *)
+  (*      var_spec "+" (λ add, iSpec τ[Z; Z] add (λ i j m, imp m {{ λ n, ⌜(n = i + j)%Z⌝ }})%I); *)
+  (*      var_spec "-" (λ sub, iSpec τ[Z; Z] sub (λ i j m, imp m {{ λ n, ⌜(n = i - j)%Z⌝ }})%I) *)
+  (*    ] {["+";"-";"*"]}. *)
+
+End ModuleSpecs.
+
+(* --------------------------------------------------------------------------*)
+(* Lemmas for resolving names. *)
+
+Section LookupName.
+
+  Lemma lookup_name_nil name :
+    lookup_name [] name = None.
+  Proof. reflexivity. Qed.
+
+  Lemma lookup_name_app_l name xs ys a :
+    lookup_name xs name = Some a →
+    lookup_name (xs ++ ys) name = Some a.
   Proof.
-    iIntros "(% & % & $)".
-    iPureIntro.
-    by apply lookup_name_app_l.
+    induction xs as [|[x v] xs IH].
+    - rewrite lookup_name_nil. discriminate 1.
+    - simpl.
+      destruct (name =? x)%string.
+      + inversion 1; by subst.
+      + apply IH.
   Qed.
 
-  Lemma var_spec_mono `{Encode A} {Φ : A → iProp Σ} (Φ' : A → iProp Σ) x η :
+  Lemma lookup_name_app_r name xs ys :
+    lookup_name xs name = None →
+    lookup_name (xs ++ ys) name = lookup_name ys name.
+  Proof.
+    induction xs as [|[x v] xs IH].
+    - auto.
+    - simpl.
+      destruct (name =? x)%string.
+      + discriminate 1.
+      + apply IH.
+  Qed.
+
+End LookupName.
+
+(* --------------------------------------------------------------------------*)
+(* Lemmas for reasoning about [in_env]. *)
+
+Section InEnv.
+  Context `{!osirisGS Σ}.
+  Context `{Encode A} {Φ : A → iProp Σ}.
+
+  Lemma in_env_mono (Φ' : A → iProp Σ) x η :
     in_env x Φ' η -∗
     (∀ a, Φ' a -∗ Φ a) -∗
     in_env x Φ η.
@@ -72,72 +137,74 @@ Section Modules.
     iApply ("Hmono" with "HΦ'").
   Qed.
 
-  Record enc_spec {PROP : Type} :=
-    has_spec
-      {
-        res_type : Type;
-        res_type_enc : Encode res_type;
-        name : var;
-        spec : res_type → PROP;
-      }.
-  (* Make it so [enc_spec] displays as [Spec name Φ]. *)
-  Global Arguments enc_spec {_}.
-  Global Arguments res_type {_}.
-  Global Arguments res_type_enc {_}.
-  Global Arguments name {_}.
-  Global Arguments spec {_}.
-  Global Arguments has_spec {_ _ _}.
-  Global Add Printing Constructor enc_spec.
+  (* [in_env] when the name [x] is found in the first of two
+     environment fragments. See the [Context] section for
+     [in_env_app_r]. *)
 
-  Instance dom_env : Dom (env) (gset var) := λ η, list_to_set (η.*1).
-
-  Definition context (specs : list (@enc_spec (iProp Σ))) d : env → iProp Σ :=
-    λ η, (⌜dom η = d⌝ ∗
-           [∗ list] s ∈ specs,
-            @in_env s.(res_type) s.(res_type_enc) s.(name) (λ res, □ s.(spec) res) η)%I.
-
-  Definition pure_context (specs : list (@enc_spec Prop)) d : env → Prop :=
-    λ η, dom η = d ∧
-         Forall (λ s,
-                   @pure_in_env s.(res_type) s.(res_type_enc) s.(name) s.(spec) η) specs.
-
-  Global Instance context_pers specs d η : Persistent (context specs d η).
-  Proof. apply _. Qed.
-
-  (*
-    Check
-    context [
-       has_spec "+" (λ add, iSpec τ[Z; Z] add (λ i j m, imp m {{ λ n, ⌜(n = i + j)%Z⌝ }})%I);
-       has_spec "-" (λ sub, iSpec τ[Z; Z] sub (λ i j m, imp m {{ λ n, ⌜(n = i - j)%Z⌝ }})%I)
-     ] {["+";"-";"*"]}.
-   *)
-
-  Lemma extract_context `{Encode A} {η} xs ys d name (spec : A → iProp Σ) :
-    context (xs ++ [has_spec name spec] ++ ys) d η -∗ in_env name spec η.
+  Lemma in_env_app_l x δ η :
+    in_env x Φ δ -∗
+    in_env x Φ (δ ++ η).
   Proof.
-    unfold context.
-    iIntros "(%Hdom & Hspecs)".
-    iPoseProof (big_sepL_app with "Hspecs") as "(_ & Hspecs)".
-    iPoseProof (big_sepL_app with "Hspecs") as "(Hspec & _)".
-    iDestruct "Hspec" as "[#Hspec _]".
-    iApply (var_spec_mono with "Hspec").
-    iIntros (res) "#Hspec'". iApply "Hspec'".
+    iIntros "(% & % & $)".
+    iPureIntro.
+    by apply lookup_name_app_l.
   Qed.
 
-  (* We immediately reduce [path_spec] to [in_env] if the path is a singleton. *)
+  (* The interaction of [in_env] and cons. *)
 
-  Lemma path_spec_singleton `{Encode A} name (Φ : A → iProp Σ) η :
-    in_env name Φ η -∗ path_spec [name] Φ η.
+  (* If the head does not match the name we are looking for,
+     we continue looking in the tail of the environment. *)
+
+  Lemma in_env_cons {η v} x y :
+    (x =? y)%string = false →
+    in_env x Φ η -∗
+    in_env x Φ ((y, v) :: η).
+  Proof.
+    iIntros (Hneq) "(%a & %Hlookup & $)".
+    iPureIntro.
+    simpl lookup_name; rewrite Hneq; apply Hlookup.
+  Qed.
+
+  (* If the head matches the name we are looking for,
+     we have to prove the postcondition over the value we have found. *)
+
+  Lemma in_env_here {η v} x y :
+    (x =? y)%string = true →
+    Φ v -∗
+    in_env x Φ ((y, #v) :: η).
+  Proof.
+    iIntros (Heq) "$".
+    iPureIntro.
+    simpl lookup_name; rewrite Heq. reflexivity.
+  Qed.
+
+End InEnv.
+
+(* --------------------------------------------------------------------------*)
+(* Lemmas for reasoning about [path_spec]. *)
+
+Section PathSpec.
+  Context `{!osirisGS Σ}.
+  Context `{Encode A} {Φ : A → iProp Σ}.
+
+  (* When the path is a singleton, proving [path_spec [x] Φ η] is
+     equivalent to proving [in_env x Φ η]. *)
+
+  Lemma path_spec_singleton x η :
+    in_env x Φ η -∗ path_spec [x] Φ η.
   Proof.
     unfold in_env.
-    iIntros "(%x & Hlookup & HΦ)".
-    iExists x. simpl. iFrame.
+    iIntros "(%v & Hlookup & HΦ)".
+    iExists v. simpl. iFrame.
   Qed.
 
-  (* If the path is a cons, we find the specification for the module
-     at the head of the path. *)
+  (* When the path is a cons, we know that the head of the path must
+     resolve to a module in the environment.
 
-  Lemma path_spec_cons {A : Type} `{Encode A} {Φ : A → iProp Σ} {η x p} mspec :
+     We will then have to resolve the tail of the path within
+     that module. *)
+
+  Lemma path_spec_cons {η x p} (mspec : env → iProp Σ) :
     in_env x mspec η -∗
     (∀ (δ : env), mspec δ -∗ path_spec p Φ δ) -∗
     path_spec (x :: p) Φ η.
@@ -150,40 +217,38 @@ Section Modules.
     - rewrite Hlookup. apply Hlookup'.
   Qed.
 
+End PathSpec.
 
-  (* If the environment is a cons, where the head does not match the
-     name we are looking for, we keep looking in the tail of the
-     environment. *)
 
-  Lemma var_spec_cons {A : Type} `{Encode A} {Φ : A → iProp Σ} {η v} x y :
-    (x =? y)%string = false →
-    in_env x Φ η -∗
-    in_env x Φ ((y, v) :: η).
+(* --------------------------------------------------------------------------*)
+(* Lemmas for exploiting [context] hypotheses to prove [in_env]. *)
+
+Section Context.
+  Context `{!osirisGS Σ}.
+  Context `{Encode A}.
+
+  (* If the pair [(x, Φ)] appears in a [context _ _ η] hypothesis,
+     then we know [in_env x Φ η]. *)
+
+  Lemma extract_context {Φ : A → iProp Σ} {η} xs ys d x :
+    context (xs ++ var_spec x Φ :: ys) d η -∗ in_env x Φ η.
   Proof.
-    iIntros (Hneq) "(%a & %Hlookup & $)".
-    iPureIntro.
-    simpl lookup_name; rewrite Hneq; apply Hlookup.
+    unfold context.
+    iIntros "(%Hdom & Hspecs)".
+    iPoseProof (big_sepL_lookup _ _ (length xs) with "Hspecs") as "HΦ".
+    { by apply list_lookup_middle. }
+    unfold var_spec.
+    iApply (in_env_mono with "HΦ").
+    iIntros (res) "#$".
   Qed.
 
-  (* If the environment is a cons, where the head does not match the
-     name we are looking for, we keep looking in the tail of the
-     environment. *)
+  (* When the name is in the second of two environment fragments
+     [η] and [δ], we can exploit a [context] hypothesis over the first
+     fragment [η] to prove that the name does not appear in [η].
 
-  Lemma var_spec_here {A : Type} `{Encode A} {Φ : A → iProp Σ} {η v} x y :
-    (x =? y)%string = true →
-    Φ v -∗
-    in_env x Φ ((y, #v) :: η).
-  Proof.
-    iIntros (Heq) "$".
-    iPureIntro.
-    simpl lookup_name; rewrite Heq. reflexivity.
-  Qed.
+     We then continue looking in the second fragment. *)
 
-  (* If the environment is an app, where the name we are looking for
-     is not in the first fragment, we keep looking in the second
-     fragment. *)
-
-  Lemma var_spec_app_r `{Encode A} {Φ : A → iProp Σ} {η x} δ d mspec :
+  Lemma in_env_app_r {Φ : A → iProp Σ} {η x} δ d mspec :
     x ∉ d →
     context mspec d δ -∗
     in_env x Φ η -∗
@@ -192,56 +257,58 @@ Section Modules.
     iIntros (Hnin) "(%Hdom & _) Hη".
     iInduction δ as [| [y v] δ ] "IH" forall (d Hnin Hdom).
     - iApply "Hη".
-    - simpl. iApply var_spec_cons.
-      + unfold dom, dom_env in Hdom. simpl in Hdom.
-        rewrite <- Hdom in Hnin.
+    - simpl. iApply in_env_cons.
+      + unfold dom, dom_env in Hdom.
+        rewrite <- Hdom in Hnin; simpl in Hnin.
         apply not_elem_of_union in Hnin as [Hnin _].
         apply not_elem_of_singleton in Hnin.
-        apply String.eqb_neq. apply Hnin.
+        by apply String.eqb_neq.
       + iApply ("IH" $! (dom δ) with "[] [//] Hη").
         iPureIntro.
-        unfold dom, dom_env in Hdom. simpl in Hdom.
-        rewrite <- Hdom in Hnin.
+        unfold dom, dom_env in Hdom.
+        rewrite <- Hdom in Hnin; simpl in Hnin.
         apply not_elem_of_union in Hnin as [_ Hnin].
         apply Hnin.
   Qed.
 
-  (* If the environment is an app, where the name we are looking for
-     is not in the first fragment, we keep looking in the second
-     fragment. *)
+  (* Proving [in_env x Φ η] when we know [context mspec d η]. *)
 
-  Lemma var_spec_app_l `{Encode A} {Φ : A → iProp Σ} {η x} δ d xs ys :
-    context (xs ++ [has_spec x Φ] ++ ys) d δ -∗
-    in_env x Φ (δ ++ η).
-  Proof.
-    iIntros "Hcontext".
-    iPoseProof (extract_context with "Hcontext") as "Hspec".
-    iApply var_spec_app. iApply "Hspec".
-  Qed.
+  (* We can either directly find the specification [Φ], or find
+     another specification [Φ'], in which case we use the monotonicity
+     over [in_env]. *)
 
-  (* We can pick out the right specification from a context. *)
-
-  Lemma var_spec_context `{Encode A} {Φ : A → iProp Σ} {x} δ d specs :
-    has_spec x Φ ∈ specs →
-    context specs d δ -∗
-    in_env x Φ δ.
+  Lemma in_env_context {Φ : A → iProp Σ} {x} η d (mspec : list (var * enc_spec)) :
+    var_spec x Φ ∈ mspec →
+    context mspec d η -∗
+    in_env x Φ η.
   Proof.
     iIntros (Hin) "Hcontext".
     apply list_elem_of_split in Hin as (l1 & l2 & ->).
     iPoseProof (extract_context with "Hcontext") as "$".
   Qed.
 
-  Lemma var_spec_context_mono `{Encode A} {Φ : A → iProp Σ} Φ' {x} δ d specs :
-    has_spec x Φ' ∈ specs →
-    context specs d δ -∗
+  Lemma in_env_context_mono {Φ : A → iProp Σ} Φ' {x} δ d mspec :
+    var_spec x Φ' ∈ mspec →
+    context mspec d δ -∗
     (∀ a, Φ' a -∗ Φ a) -∗
     in_env x Φ δ.
   Proof.
     iIntros (Hin) "Hcontext Hmono".
     apply list_elem_of_split in Hin as (l1 & l2 & ->).
     iPoseProof (extract_context with "Hcontext") as "Hspec".
-    iApply (var_spec_mono with "Hspec Hmono").
+    iApply (in_env_mono with "Hspec Hmono").
   Qed.
+
+End Context.
+
+Section PathRule.
+  Context `{!osirisGS Σ}.
+
+  (* Using [path_spec] defined above, we prove a new reasoning rule
+     for paths lookups in the environment.
+
+     The end-user should never see [path_spec], and we should trive
+     to automatically discharge that proof obligation in all cases. *)
 
   Lemma imp_EPath_spec {E : coPset} {Ψ : iEff Σ} {A : Type} {EncA : Encode A}
     {Φ : A → iProp Σ} {ζ : exn → iProp Σ} (η : env) (p : path) :
@@ -255,22 +322,35 @@ Section Modules.
     iExists x; auto.
   Qed.
 
-  Lemma imp_EPath_var {E Ψ ζ} {A : Type} `{Encode A} {η p} (a : A) :
-    lookup_path η p = Some #a →
-    ⊢ imp (eval η (EPath p)) @ E <|Ψ|> ⟨⟨ ζ ⟩⟩ {{ λ a', ⌜a' = a⌝ }}.
-  Proof.
-    iIntros (Hlookup).
-    iApply imp_EPath; eauto.
-  Qed.
+End PathRule.
 
-End Modules.
-
+(* --------------------------------------------------------------------------*)
 (* --------------------------------------------------------------------------*)
 (* Implementing the [imp_path] tactic. *)
 
 From Ltac2 Require Import Ltac2 Printf Bool.
 
-Ltac2 get_env_spec (η : constr) :=
+(** Fetching hypotheses in the iris context. *)
+
+(* [is_arg_of arg t] checks if [t] is an application, and if it is,
+   checks whether [arg] is an argument of that application.
+
+   We use it to check whether a hypothesis mentions a given term. *)
+
+Ltac2 is_arg_of (arg : constr) (t : constr) : bool :=
+  match Constr.Unsafe.kind t with
+  | Constr.Unsafe.App _ tail =>
+      Array.mem Constr.equal arg tail
+  | _ => false
+  end.
+
+(* [get_env_spec η] takes an environment fragment [η] and tries to
+   find a hypothesis of the form [context _ _ η] in the iris context.
+
+   If found, it returns the name (a Gallina term of type [base.ident])
+   of that hypothesis. *)
+
+Ltac2 get_env_spec (η : constr) : constr :=
   let (pers_hyps, spat_hyps) := get_iris_hyps () in
   let rec go env :=
     lazy_match! env with
@@ -279,17 +359,23 @@ Ltac2 get_env_spec (η : constr) :=
                         (Some (fprintf "Could not find [context] specification for environment %t" η)))
     | environments.Esnoc ?env ?name ?prop =>
         match! prop with
-        | env_lookups.context ?_specs ?_domain ?δ =>
+        | env_lookups.context _ _ ?δ =>
             if Constr.equal η δ then
               name
             else
               go env
-        | ?_spec ?δ =>
-            if Constr.equal η δ then
-              name
-            else
-              go env
-        | _ => go env
+        | _ =>
+            (* If we [η] appears as an argument of the hypothesis
+               (this occurs when the module specification is behind a definition). *)
+            if is_arg_of η prop then
+              (* We try to unify the hypothesis with [context _ _ η],
+                 if successfull, we return the hypothesis' name *)
+              Control.plus
+                (fun _ =>
+                   Std.unify prop open_constr:(env_lookups.context _ _ $η);
+                   name)
+                (fun _ => go env)
+            else go env
         end
     end
   in
@@ -297,7 +383,12 @@ Ltac2 get_env_spec (η : constr) :=
     (fun _ => go pers_hyps)
     (fun _ => go spat_hyps).
 
-Ltac2 get_var_spec (x : constr) (η : constr) :=
+
+(* [get_in_env x η] takes a name [x] and an environment fragment [η]
+   and tries to find a hypothesis fo the form [in_env x _ η] in the
+   iris context. *)
+
+Ltac2 get_in_env (x : constr) (η : constr) : constr :=
   let (pers_hyps, spat_hyps) := get_iris_hyps () in
   let rec go env :=
     lazy_match! env with
@@ -306,7 +397,7 @@ Ltac2 get_var_spec (x : constr) (η : constr) :=
                         (Some (fprintf "Could not find [in_env] specification for name %t" x)))
     | environments.Esnoc ?env ?name ?prop =>
         match! prop with
-        | in_env ?y ?_spec ?δ =>
+        | in_env ?y _ ?δ =>
             if Constr.equal x y && Constr.equal η δ then
               name
             else
@@ -320,71 +411,117 @@ Ltac2 get_var_spec (x : constr) (η : constr) :=
     (fun _ => go spat_hyps).
 
 
-Ltac2 var_spec_cons () :=
-  iApply var_spec_cons; Control.focus 1 1 (fun _ => reflexivity).
+(** Applying lemmas that reason about [in_env]. *)
 
-Ltac2 var_spec_here () :=
-  iApply var_spec_here; Control.focus 1 1 (fun _ => reflexivity).
+(* These lemmas often come with side-conditions.
+   The tactics fails if those side conditions cannot be solved. *)
 
-Ltac2 var_spec_app_r (hyp : constr) :=
-  iApply (var_spec_app_r with $hyp);
+Ltac2 in_env_cons () :=
+  iApply in_env_cons;
+  (* For this tactic to succeed, it must solve the [x =? y = false]
+     condiction of the [in_env_cons] lemma. *)
+  Control.focus 1 1 (fun _ => reflexivity).
+
+Ltac2 in_env_here () :=
+  iApply in_env_here;
+  (* For this tactic to succeed, it must solve the [x =? y = true]
+     condition of [in_env_here]. *)
+  Control.focus 1 1 (fun _ => reflexivity).
+
+Ltac2 in_env_app_l () :=
+  iApply in_env_app_l.
+
+Ltac2 in_env_app_r (hyp : constr) :=
+  iApply (in_env_app_r with $hyp);
+  (* For this tactic to succeed, it must solve the [x ∉ d] condition
+     of [in_env_app_r]. *)
   Control.focus 1 1 (fun _ => complete (fun _ => ltac1:(set_solver))).
 
-Ltac2 var_spec_app () :=
-  iApply var_spec_app.
-
-Ltac2 var_spec_context hyp :=
+Ltac2 in_env_context hyp :=
   Control.plus
     (fun _ =>
-       iApply (var_spec_context with $hyp);
+       iApply (in_env_context with $hyp);
+       (* For this branch of the tactic to succeed, it must solve the
+          [var_spec x Φ ∈ mspec] condition of [in_env_context] *)
        complete (fun _ => repeat constructor))
+    (* If the previous branch of the tactic failed,
+       try again with the monotonic variant of the lemma. *)
     (fun _ =>
-       iApply (var_spec_context_mono with $hyp) >
+       iApply (in_env_context_mono with $hyp) >
+         (* Note that the first condition must still succeed, but we
+            are allowed to fail to discharge the monotonicity
+            condition, which then becomes a proof obligation for the
+            user. *)
          [  complete (fun _ => repeat constructor) | auto ]).
 
-Ltac2 rec solve_var_spec () :=
+
+(** Solving environment lookup goals. *)
+
+(* [solve_in_env ()] solves a goal of the form [in_env x Φ η]. *)
+
+(*
+   It works by matching on the shape of [η], proceeding as follows:
+
+   - if [η] is a cons: apply either [in_env_here] or [in_env_cons].
+   - if [η] is an app: apply either [in_env_app_r] or [in_env_app_l].
+   - otherwise: try and find a hypothesis on [η] in the context.
+*)
+
+Ltac2 rec solve_in_env () :=
   lazy_match! get_iris_goal () with
   | in_env ?name ?_spec ?env =>
+      (* We use [match!] instead of [lazy_match!] so that we always
+         fall back to the last branch in case we have a hypothesis
+         over an environment which is an app or a cons. *)
       match! env with
       | (?name', ?_val) :: _ =>
           if Constr.equal name name' then
-            var_spec_here ()
+            in_env_here ()
           else
-            (var_spec_cons ();
-             Control.enter solve_var_spec)
-      | ?δ ++ ?_η =>
+            (in_env_cons ();
+             Control.enter solve_in_env)
+      | ?δ ++ _ =>
           Control.plus
             (fun _ =>
                let spec_name := get_env_spec δ in
-               var_spec_app_r spec_name;
-               last solve_var_spec)
+               in_env_app_r spec_name;
+               Control.enter solve_in_env)
             (fun _ =>
-               var_spec_app ();
-               solve_var_spec ())
+               in_env_app_l ();
+               solve_in_env ())
       | ?η =>
           Control.plus
+            (* Try to find a corresponding [in_env] hypothesis. *)
             (fun _ =>
-               let spec_name := get_var_spec name η in
-               iApply (var_spec_mono with $spec_name);
+               let spec_name := get_in_env name η in
+               iApply (in_env_mono with $spec_name);
                let ha := iFresh "ha" in
                iIntros ("% " ++ $ha)%string; try (iApply $ha))
             (fun _ =>
                Control.plus
+                 (* Try to find a corresponding [context] hypothesis. *)
                  (fun _ =>
                     let spec_name := get_env_spec η in
-                    var_spec_context spec_name)
+                    in_env_context spec_name)
                  (fun _ =>
                     Control.zero (Tactic_failure
-                                    (Some (fprintf "Could not solve goal [var_spec %t _ %t]" name env)))))
+                                    (Some (fprintf "Could not solve goal [in_env %t _ %t]" name env)))))
       end
-  | _ => Control.zero (Tactic_failure (Some (fprintf "Expected goal to be [path_spec]")))
+  | _ => Control.zero (Tactic_failure (Some (fprintf "Expected goal to be [in_env]")))
   end.
+
+(* [path_spec_to_in_env] takes a goal of the form [path_spec p Φ η]
+   and reduces it to a goal of the form [in_env _ _ η] by applying
+   either [path_spec_singleton] or [path_spec_cons]. *)
+
+(* We use the [detected_path] type as a return type for
+   [path_spec_to_in_env] to indicate which choice was made. *)
 
 Ltac2 Type detected_path :=
   [ | Psingleton
     | Pcons ].
 
-Ltac2 rec path_spec_to_var_spec () :=
+Ltac2 rec path_spec_to_in_env () : detected_path :=
   lazy_match! get_iris_goal () with
   | path_spec ?path ?_spec ?_env =>
       match! path with
@@ -398,15 +535,26 @@ Ltac2 rec path_spec_to_var_spec () :=
   | _ => Control.zero (Tactic_failure (Some (fprintf "Expected goal to be [path_spec]")))
   end.
 
+(* [solve_path_spec] solves a goal of the form [path_spec p Φ η]. *)
+
+(* It first calls [path_spec_to_in_env] to produce a subgoal of the
+   form [in_env _ _ η], before calling [solve_in_env] to solve that
+   subgoal.
+
+   In the case where the path is not a singleton, [solve_path_spec]
+   calls itself recursively on the tail of the path. *)
+
 Ltac2 rec solve_path_spec () :=
-  match path_spec_to_var_spec () with
-  | Psingleton => solve_var_spec ()
+  match path_spec_to_in_env () with
+  | Psingleton => solve_in_env ()
   | Pcons =>
-      Control.focus 1 1 (fun _ => complete solve_var_spec);
+      Control.focus 1 1 (fun _ => complete solve_in_env);
       let hyp_name := iFresh "Hpath" in
       iIntros ("% #" ++ $hyp_name)%string;
       solve_path_spec ()
   end.
+
+(** User-level tactics. *)
 
 Ltac2 solve_eq_goal () :=
   lazy_match! get_iris_goal () with
@@ -485,18 +633,18 @@ Section TacticTests.
   Definition sub_spec sub : iProp Σ := □ iSpec τ[Z;Z] sub (λ (i j : Z) m, imp m {{ λ k, ⌜(k = i - j)%Z⌝ }})%I.
   Definition a_spec a : iProp Σ := ∀ (A : Type), □ ⌜a > 2⌝.
 
-  Definition module3_spec η := context [has_spec "sub" sub_spec] {["sub"]} η.
-  Definition module2_spec η := context [has_spec "Module3" module3_spec] {["Module3"; "some"; "other"; "stuff"]} η.
+  Definition module3_spec η := context [var_spec "sub" sub_spec] {["sub"]} η.
+  Definition module2_spec η := context [var_spec "Module3" module3_spec] {["Module3"; "some"; "other"; "stuff"]} η.
 
   Lemma example_proof δ η :
     in_env "z" (λ (i : Z), ⌜i > 0⌝) η -∗
     in_env "a" a_spec η -∗
-    context [has_spec
+    context [var_spec
                "Module1"
-               (context [has_spec "some_other_val" (λ (_ : val), True);
-                         has_spec "add" add_spec] {["some_other_val";"add"]})
+               (context [var_spec "some_other_val" (λ (_ : val), True);
+                         var_spec "add" add_spec] {["some_other_val";"add"]})
       ] {["Module1"]} δ -∗
-    context [has_spec "Module2" module2_spec] {["Module2";"z"]} η -∗
+    context [var_spec "Module2" module2_spec] {["Module2";"z"]} η -∗
     imp (eval (δ ++ η) e) {{ λ (i : Z), ⌜i > 0⌝ }}.
   Proof.
     iIntros "#zspec #aspec #δspec #ηspec".
